misc.v
@@ -1,0 +1,88 @@
+Require Import ssreflect ssrnat seq ssrbool eqtype.
+
+Set Implicit Arguments.
+
+Lemma ltn_trans_tight m n p : m < n -> n < p -> m < p.-1.
+Proof. elim: p n m => [|p IHp ] n m.
+  by [].
+move => H0. rewrite leq_eqVlt => /orP [].
+  move/eqP => <-. exact: H0.
+rewrite ltnS => H1. move: (IHp _ _ H0 H1) => /=.
+case: p IHp H1 => [|p] IHp H1.
+  by [].
+by exact: ltnW.
+Qed.
+
+Lemma ltn_trans_tight' m n p : m < n -> n < p.-1 -> m < p.-1.
+Proof. elim: p n m => [|p IHp ] n m.
+  by [].
+move => H0. rewrite leq_eqVlt => /orP [].
+  move/eqP => <-. apply: leqW. by [].
+move/leqW. apply: ltn_trans_tight. by apply: leqW.
+Qed.
+
+Lemma size_induction (X : Type) (f : X -> nat) (p: X ->Prop) :
+( forall x, ( forall y, f y < f x -> p y) -> p x) -> forall x, p x.
+Proof. intros A x. apply A. induction (f x). by [].
+intros y B. apply A. intros z C. apply IHn.
+move: C B. apply: ltn_trans_tight. Qed.
+
+(* seq X helpers. *)
+Section Seq.
+
+Variable X: Type.
+  
+Lemma size_take_bound (w: seq X) n : size (take n w) <= size w.
+Proof. elim: n w => [|n IHn] w.
+  by rewrite take0.
+rewrite size_take.
+case_eq (n.+1 < size w).
+  apply: leq_trans. apply: leqW. exact: ltnSn.
+by [].
+Qed.
+
+Lemma size_take_bound' (w: seq X) n : size (take n w) <= n.
+Proof. elim: n w => [|n IHn] w.
+  by rewrite take0.
+rewrite size_take.
+case_eq (n.+1 < size w).
+  move => _. exact: ltnSn.
+move/negbT. by rewrite -leqNgt.
+Qed.
+
+Lemma size_take_underflow (w: seq X) n : size (take n w) < n -> size w < n.
+Proof. elim: n w => [|n IHn] w.
+  by rewrite take0.
+rewrite size_take.
+case_eq (n.+1 < size w).
+  move => _. by rewrite ltnn.
+move/negbT. by rewrite -leqNgt.
+Qed.
+
+Lemma take_undersize (w: seq X) n k : n <= k -> take n (take k w) = take n w.
+Proof. elim: w k n => [|a w IHw] k n.
+  by [].
+rewrite take_cons. destruct k. 
+  by rewrite leqn0 => /eqP ->.
+rewrite take_cons. destruct n.
+  by [].
+move => H0. rewrite IHw.
+  by [].
+move: H0. rewrite -{1}(addn1 n) -(addn1 k).
+by rewrite leq_add2r.
+Qed.
+
+Lemma take_oversizeS (w: seq X) n: size w < n -> take n w = take n.-1 w.
+Proof. move: w n. apply: last_ind => [|w a IHw] n.
+  by [].
+rewrite -cats1 => H0. rewrite take_oversize.
+  rewrite take_oversize.
+    by [].
+  destruct n.
+    by [].
+  by [].
+exact: ltnW.
+Qed.
+
+Lemma take_oversize_trans (w: seq X) n k : size w < n -> n < k -> take n w = take k w
+End Seq.
